Move auxiliary theorems to {chor,endpoint,payload}Props

semantics/proofs/endpointPropsScript.sml
@@ -2019,4 +2019,76 @@ Proof
   simp[GSYM o_DEF] \\ metis_tac[o_ASSOC,MAP_ZIP]
 QED
 
+(* Makes sure a network has every message queue empty (epn version) *)
+Definition empty_q_def:
+  empty_q  NNil = T
+∧ empty_q (NPar n1 n2)     = (empty_q n1 ∧ empty_q n2)
+∧ empty_q (NEndpoint _ s _) = (s.queue = [])
+End
+
+(* If all queues are empty a network is only queue congruent (qcong)
+   with itself (epn version)
+*)
+Theorem empty_queue_qcong:
+  ∀epn epn'.
+   qcong epn epn' ∧
+   empty_q epn
+   ⇒ epn' = epn
+Proof
+  Induct
+  \\ ONCE_REWRITE_TAC [qcong_cases] \\ rw [empty_q_def]
+  >- (metis_tac [qcong_rules,qcong_nil_rel_nil])
+  >- (metis_tac [qcong_rules,qcong_nil_rel_nil])
+  >- (drule qcong_par_rel_par_sym \\ rw []
+      \\ imp_res_tac qcong_sym
+      \\ fs [])
+  >- (drule_then drule qcong_trans
+      \\ disch_then (mp_then Any mp_tac qcong_par_rel_par)
+      \\ rw [])
+  >- (drule qcong_sym
+      \\ disch_then (mp_then Any mp_tac qcong_endpoint_rel_endpoint)
+      \\ rw [] \\ drule qcong_IMP_qrel
+      \\ rw [] \\ drule qrel_LENGTH \\ rw []
+      \\ rw [state_component_equality]
+      \\ drule qcong_bindings_eq \\ fs [])
+  >- (drule_then drule qcong_trans
+      \\ disch_then (mp_then Any mp_tac qcong_endpoint_rel_endpoint)
+      \\ rw [] \\ drule_then drule qcong_trans
+      \\ rw [] \\ drule qcong_IMP_qrel
+      \\ rw [] \\ drule qrel_LENGTH \\ rw []
+      \\ rw [state_component_equality]
+      \\ drule qcong_bindings_eq \\ fs [])
+  \\ fs []
+QED
+
+(* If a network is empty_q it can only be junkcong with
+   other empty_q networks *)
+Theorem empty_q_junkcong:
+  ∀epn fv epn'. junkcong fv epn epn' ∧ empty_q epn
+  ⇒ empty_q epn'
+Proof
+  Induct
+  \\ ONCE_REWRITE_TAC [junkcong_cases]
+  \\ rw [empty_q_def]
+  \\ rw [empty_q_def]
+  >- metis_tac[empty_q_def,junkcong_nil_rel_nil,junkcong_sym]
+  >- metis_tac[empty_q_def,junkcong_nil_rel_nil,junkcong_sym]
+  >- (drule junkcong_sym
+      \\ disch_then (mp_then Any mp_tac junkcong_par_rel_par)
+      \\ rw [] \\ fs [empty_q_def] \\ metis_tac [])
+  >- (drule_then drule junkcong_trans
+      \\ disch_then (mp_then Any mp_tac junkcong_par_rel_par)
+      \\ rw [] \\ fs [empty_q_def] \\ metis_tac [])
+  >- metis_tac []
+  >- metis_tac []
+  >- (drule junkcong_sym
+      \\ disch_then (mp_then Any mp_tac junkcong_endpoint_rel_endpoint)
+      \\ rw [] \\ rw [empty_q_def]
+      \\ drule junkcong_endpoint_queue_eq \\ fs [])
+  \\ drule_then (drule_then assume_tac) junkcong_trans
+  \\ drule junkcong_endpoint_rel_endpoint
+  \\ rw [] \\ rw [empty_q_def]
+  \\ drule junkcong_endpoint_queue_eq \\ fs []
+QED
+
 val _ = export_theory ()
